First round of cleanup for SepAuto.

HOL/SepLogic/SepAuto.thy
@@ -1,146 +1,126 @@
+(* The development here follows Separation_Logic_Imperative_HOL
+   (by Lammich and Meis) in the AFP *)
+
 theory SepAuto
-imports "../Auto2_Main" "~~/src/HOL/Imperative_HOL/Imperative_HOL"
-keywords "@hoare_induct" :: prf_decl % "proof"
+  imports "../Auto2_Main" "~~/src/HOL/Imperative_HOL/Imperative_HOL"
+  keywords "@hoare_induct" :: prf_decl % "proof"
 begin
 
-subsection {* Partial Heaps *}
-text {*
-  A partial heap is modeled by a heap and a set of valid addresses, with the
-  side condition that the valid addresses have to be within the limit of the
-  heap. This modeling is somewhat strange for separation logic, however, it 
-  allows us to solve some technical problems related to definition of 
-  Hoare triples, that will be detailed later.
-*}
+section {* Partial Heaps *}
+
 type_synonym pheap = "heap \<times> addr set"
 
-text {* Predicate that expresses that the address set of a partial heap is 
-  within the heap's limit.
-*}
 fun in_range :: "(heap \<times> addr set) \<Rightarrow> bool" where
   "in_range (h,as) \<longleftrightarrow> (\<forall>a\<in>as. a < lim h)"
 setup {* add_rewrite_rule @{thm in_range.simps} *}
 
-text {* Relation that holds if two heaps are identical on a given 
-  address range. *}
-definition relH :: "addr set \<Rightarrow> heap \<Rightarrow> heap \<Rightarrow> bool" where
+(* Two heaps agree on a set of addresses. *)
+definition relH :: "addr set \<Rightarrow> heap \<Rightarrow> heap \<Rightarrow> bool" where [rewrite]:
   "relH as h h' = (in_range (h, as) \<and> in_range (h', as) \<and>
-     (\<forall>t. \<forall>a \<in> as. refs h t a = refs h' t a \<and> arrays h t a = arrays h' t a))"
-setup {* add_rewrite_rule @{thm relH_def} *}
+     (\<forall>t. \<forall>a\<in>as. refs h t a = refs h' t a \<and> arrays h t a = arrays h' t a))"
 
-lemma relH_dist_union [forward]: "relH (as \<union> as') h h' \<Longrightarrow> relH as h h' \<and> relH as' h h'" by auto2
+lemma relH_dist_union [forward]:
+  "relH (as \<union> as') h h' \<Longrightarrow> relH as h h' \<and> relH as' h h'" by auto2
 
-lemma relH_ref [rewrite]: "relH as h h' \<Longrightarrow> addr_of_ref r \<in> as \<Longrightarrow> Ref.get h r = Ref.get h' r"
+lemma relH_ref [rewrite]:
+  "relH as h h' \<Longrightarrow> addr_of_ref r \<in> as \<Longrightarrow> Ref.get h r = Ref.get h' r"
   by (simp add: Ref.get_def relH_def)
 
-lemma relH_array [rewrite]: "relH  as h h' \<Longrightarrow> addr_of_array r \<in> as \<Longrightarrow> Array.get h r = Array.get h' r"
+lemma relH_array [rewrite]:
+  "relH as h h' \<Longrightarrow> addr_of_array r \<in> as \<Longrightarrow> Array.get h r = Array.get h' r"
   by (simp add: Array.get_def relH_def)
 
-lemma relH_set_ref [resolve]: "relH {a. a < lim h \<and> a \<notin> {addr_of_ref r}} h (Ref.set r x h)"
+lemma relH_set_ref [resolve]:
+  "relH {a. a < lim h \<and> a \<notin> {addr_of_ref r}} h (Ref.set r x h)"
   by (simp add: Ref.set_def relH_def)
 
-lemma relH_set_array [resolve]: "relH {a. a < lim h \<and> a \<notin> {addr_of_array r}} h (Array.set r x h)"
+lemma relH_set_array [resolve]:
+  "relH {a. a < lim h \<and> a \<notin> {addr_of_array r}} h (Array.set r x h)"
   by (simp add: Array.set_def relH_def)
 
-subsection {* Assertions *}
-text {*
-  Assertions are predicates on partial heaps, that fulfill a well-formedness 
-  condition called properness: They only depend on the part of the heap
-  by the address set, and must be false for partial heaps that are not in range.
-*}
+section {* Assertions *}
+
 datatype assn_raw = Assn (assn_fn: "pheap \<Rightarrow> bool")
-setup {* add_forward_prfstep @{thm assn_raw.expand} *}
 
 fun aseval :: "assn_raw \<Rightarrow> pheap \<Rightarrow> bool" where
   "aseval (Assn f) h = f h"
 setup {* add_rewrite_rule @{thm aseval.simps} *}
 
-definition proper :: "assn_raw \<Rightarrow> bool" where
+definition proper :: "assn_raw \<Rightarrow> bool" where [rewrite]:
   "proper P = (
     (\<forall>h as. aseval P (h,as) \<longrightarrow> in_range (h,as)) \<and>
     (\<forall>h h' as. aseval P (h,as) \<longrightarrow> relH as h h' \<longrightarrow> in_range (h',as) \<longrightarrow> aseval P (h',as)))"
-setup {* add_rewrite_rule @{thm proper_def} *}
+setup {* add_property_const @{term proper} *}
 
 typedef assn = "Collect proper"
 @proof @have "Assn in_range \<in> Collect proper" @qed
 
-setup {* add_resolve_prfstep (equiv_forward_th @{thm Rep_assn_inject}) *}
+setup {* add_rewrite_rule @{thm Rep_assn_inject} *}
+setup {* register_wellform_data ("Abs_assn P", ["proper P"]) *}
+setup {* add_prfstep_check_req ("Abs_assn P", "proper P") *}
 
-theorem Abs_assn_inverse' [rewrite]: "proper y \<Longrightarrow> Rep_assn (Abs_assn y) = y"
+lemma Abs_assn_inverse' [rewrite]: "proper y \<Longrightarrow> Rep_assn (Abs_assn y) = y"
   by (simp add: Abs_assn_inverse)
 
-theorem proper_Rep_assn: "proper (Rep_assn P)" using Rep_assn by auto
-setup {* add_forward_prfstep_cond @{thm proper_Rep_assn} [with_term "Rep_assn ?P"] *}
+lemma proper_Rep_assn [forward]: "proper (Rep_assn P)" using Rep_assn by auto
 
-definition models :: "pheap \<Rightarrow> assn \<Rightarrow> bool" (infix "\<Turnstile>" 50) where
-  "h \<Turnstile> P = aseval (Rep_assn P) h"
-setup {* add_rewrite_rule_bidir @{thm models_def} *}
+definition models :: "pheap \<Rightarrow> assn \<Rightarrow> bool" (infix "\<Turnstile>" 50) where [rewrite_bidir]:
+  "h \<Turnstile> P \<longleftrightarrow> aseval (Rep_assn P) h"
 
 lemma models_in_range [resolve]: "h \<Turnstile> P \<Longrightarrow> in_range h" by auto2
 
-lemma mod_relH [forward]:
-  "relH as h h' \<Longrightarrow> (h, as) \<Turnstile> P \<Longrightarrow> (h', as) \<Turnstile> P" by auto2
-
-setup {* add_gen_prfstep ("proper_assn_case",
-  [WithTerm @{term_pat "?h \<Turnstile> Abs_assn ?P"},
-   CreateCase @{term_pat "proper ?P"}]) *}
+lemma mod_relH [forward]: "relH as h h' \<Longrightarrow> (h, as) \<Turnstile> P \<Longrightarrow> (h', as) \<Turnstile> P" by auto2
 
 instantiation assn :: one begin
-  definition one_assn :: assn where "1 \<equiv> Abs_assn (Assn (\<lambda>h. snd h = {}))"
+definition one_assn :: assn where [rewrite]:
+  "1 \<equiv> Abs_assn (Assn (\<lambda>h. snd h = {}))"
 instance .. end
 
 abbreviation one_assn :: assn ("emp") where "one_assn \<equiv> 1"
 
-setup {* add_rewrite_rule (to_obj_eq_th @{thm one_assn_def}) *}
-theorem one_assn_rule [rewrite]: "h \<Turnstile> emp \<longleftrightarrow> snd h = {}" by auto2
+lemma one_assn_rule [rewrite]: "h \<Turnstile> emp \<longleftrightarrow> snd h = {}" by auto2
 setup {* del_prfstep_thm @{thm one_assn_def} *}
 
-definition set_partition :: "'a set \<Rightarrow> 'a set \<Rightarrow> 'a set \<Rightarrow> bool" where
+definition set_partition :: "'a set \<Rightarrow> 'a set \<Rightarrow> 'a set \<Rightarrow> bool" where [rewrite]:
   "set_partition S T1 T2 = (S = T1 \<union> T2 \<and> T1 \<inter> T2 = {})"
-setup {* add_rewrite_rule @{thm set_partition_def} *}
 
 instantiation assn :: times begin
-  definition times_assn where
-    "P * Q = Abs_assn (Assn (
-      \<lambda>h. (\<exists>as1 as2. set_partition (snd h) as1 as2 \<and>
-                     aseval (Rep_assn P) (fst h, as1) \<and> aseval (Rep_assn Q) (fst h, as2))))"
+definition times_assn where [rewrite]:
+  "P * Q = Abs_assn (Assn (
+    \<lambda>(h, as). (\<exists>as1 as2. set_partition as as1 as2 \<and>
+                   aseval (Rep_assn P) (h, as1) \<and> aseval (Rep_assn Q) (h, as2))))"
 instance .. end
 
-setup {* add_rewrite_rule @{thm times_assn_def} *}
 lemma mod_star_conv [rewrite]:
-  "h \<Turnstile> A * B \<longleftrightarrow>
-    (\<exists>as1 as2. set_partition (snd h) as1 as2 \<and> (fst h, as1) \<Turnstile> A \<and> (fst h, as2) \<Turnstile> B)" by auto2
+  "(h, as) \<Turnstile> A * B \<longleftrightarrow> (\<exists>as1 as2. set_partition as as1 as2 \<and> (h, as1) \<Turnstile> A \<and> (h, as2) \<Turnstile> B)" by auto2
 setup {* del_prfstep_thm @{thm times_assn_def} *}
 
-definition entails :: "assn \<Rightarrow> assn \<Rightarrow> bool" (infix "\<Longrightarrow>\<^sub>A" 10) where
-  "(P \<Longrightarrow>\<^sub>A Q) \<longleftrightarrow> (\<forall>h. h \<Turnstile> P \<longrightarrow> h \<Turnstile> Q)"
-setup {* add_backward_prfstep (equiv_backward_th @{thm entails_def}) *}
-
-lemma entailsD [forward]:
-  "P \<Longrightarrow>\<^sub>A Q \<Longrightarrow> h \<Turnstile> P \<Longrightarrow> h \<Turnstile> Q" using entails_def by blast
-
-theorem aseval_ext [backward]: "\<forall>h. aseval P h = aseval P' h \<Longrightarrow> P = P'"
+lemma aseval_ext [backward]: "\<forall>h. aseval P h = aseval P' h \<Longrightarrow> P = P'"
   apply (cases P) apply (cases P') by auto
 
-lemma ent_iffI: "(A \<Longrightarrow>\<^sub>A B) \<and> (B \<Longrightarrow>\<^sub>A A) \<Longrightarrow> A = B"
-@proof @have "Rep_assn A = Rep_assn B" @qed
-setup {* add_backward_prfstep_cond @{thm ent_iffI} [with_filt (order_filter "A" "B")] *}
+lemma assn_ext: "\<forall>h as. (h, as) \<Turnstile> P \<longleftrightarrow> (h, as) \<Turnstile> Q \<Longrightarrow> P = Q"
+@proof @have "Rep_assn P = Rep_assn Q" @qed
+setup {* add_backward_prfstep_cond @{thm assn_ext} [with_filt (order_filter "P" "Q")] *}
+
 setup {* del_prfstep_thm @{thm aseval_ext} *}
 
-theorem assn_one_left: "1 * P = (P::assn)"
+lemma assn_one_left: "1 * P = (P::assn)"
 @proof
-  @have "\<forall>h. h \<Turnstile> P \<longrightarrow> h \<Turnstile> 1 * P" @with @have "set_partition (snd h) {} (snd h)" @end
+  @have "\<forall>h as. (h, as) \<Turnstile> P \<longleftrightarrow> (h, as) \<Turnstile> 1 * P" @with
+    @have "set_partition as {} as"
+  @end
 @qed
 
-theorem set_partition_comm [forward]: "set_partition S T1 T2 \<Longrightarrow> set_partition S T2 T1" by auto2
+lemma set_partition_comm [forward]:
+  "set_partition S T1 T2 \<Longrightarrow> set_partition S T2 T1" by auto2
 
-theorem assn_times_comm: "P * Q = Q * (P::assn)" by auto2
+lemma assn_times_comm: "P * Q = Q * (P::assn)" by auto2
 
-theorem set_partition_assoc [forward]:
+lemma set_partition_assoc [forward]:
   "set_partition S T1 T2 \<Longrightarrow> set_partition T1 T11 T12 \<Longrightarrow>
    set_partition S T11 (T12 \<union> T2) \<and> set_partition (T12 \<union> T2) T12 T2" by auto2
 
-setup {* del_prfstep_thm @{thm models_def} *}
-theorem assn_times_assoc: "(P * Q) * R = P * (Q * (R::assn))" by auto2
+lemma assn_times_assoc: "(P * Q) * R = P * (Q * (R::assn))" by auto2
 setup {* del_prfstep_thm @{thm set_partition_comm} *}
 setup {* del_prfstep_thm @{thm set_partition_assoc} *}
 
@@ -149,113 +129,123 @@ instantiation assn :: comm_monoid_mult begin
   apply (rule assn_times_assoc) apply (rule assn_times_comm) by (rule assn_one_left)
 end
 
-subsubsection {* Existential Quantification *}
+subsection {* Existential Quantification *}
 
-definition ex_assn :: "('a \<Rightarrow> assn) \<Rightarrow> assn" (binder "\<exists>\<^sub>A" 11) where
+definition ex_assn :: "('a \<Rightarrow> assn) \<Rightarrow> assn" (binder "\<exists>\<^sub>A" 11) where [rewrite]:
   "(\<exists>\<^sub>Ax. P x) = Abs_assn (Assn (\<lambda>h. \<exists>x. h \<Turnstile> P x))"
-setup {* add_rewrite_rule @{thm ex_assn_def} *}
 
-setup {* add_rewrite_rule_bidir @{thm models_def} *}
 lemma mod_ex_dist [rewrite]: "(h \<Turnstile> (\<exists>\<^sub>Ax. P x)) \<longleftrightarrow> (\<exists>x. h \<Turnstile> P x)" by auto2
-setup {* del_prfstep_thm @{thm models_def} *}
+setup {* del_prfstep_thm @{thm ex_assn_def} *}
 
 lemma ex_distrib_star: "(\<exists>\<^sub>Ax. P x * Q) = (\<exists>\<^sub>Ax. P x) * Q"
 @proof
-  @have "\<forall>h. h \<Turnstile> (\<exists>\<^sub>Ax. P x) * Q \<longrightarrow> h \<Turnstile> (\<exists>\<^sub>Ax. P x * Q)" @with
-    @obtain as1 as2 where "set_partition (snd h) as1 as2" "(fst h, as1) \<Turnstile> (\<exists>\<^sub>Ax. P x) \<and> (fst h, as2) \<Turnstile> Q"
-    @obtain x where "(fst h, as1) \<Turnstile> P x"
-    @have "h \<Turnstile> P x * Q"
+  @have "\<forall>h as. (h, as) \<Turnstile> (\<exists>\<^sub>Ax. P x) * Q \<longleftrightarrow> (h, as) \<Turnstile> (\<exists>\<^sub>Ax. P x * Q)" @with
+    @case "(h, as) \<Turnstile> (\<exists>\<^sub>Ax. P x) * Q" @with
+      @obtain as1 as2 where "set_partition as as1 as2" "(h, as1) \<Turnstile> (\<exists>\<^sub>Ax. P x)" "(h, as2) \<Turnstile> Q"
+      @obtain x where "(h, as1) \<Turnstile> P x"
+      @have "(h, as) \<Turnstile> P x * Q"
+    @end
   @end
 @qed
 
-subsubsection {* Pointers *}
+subsection {* Pointers *}
 
-text {* In Imperative HOL, we have to distinguish between pointers to single
-  values and pointers to arrays. For both, we define assertions that 
-  describe the part of the heap that a pointer points to. *}
-
-definition sngr_assn :: "'a::heap ref \<Rightarrow> 'a \<Rightarrow> assn" (infix "\<mapsto>\<^sub>r" 82) where
+definition sngr_assn :: "'a::heap ref \<Rightarrow> 'a \<Rightarrow> assn" (infix "\<mapsto>\<^sub>r" 82) where [rewrite]:
   "r \<mapsto>\<^sub>r x = Abs_assn (Assn (
-    \<lambda>h. Ref.get (fst h) r = x \<and> snd h = {addr_of_ref r} \<and> addr_of_ref r < lim (fst h)))"
+    \<lambda>(h, as). Ref.get h r = x \<and> as = {addr_of_ref r} \<and> addr_of_ref r < lim h))"
 
-setup {* add_rewrite_rule_bidir @{thm models_def} *}
-setup {* add_rewrite_rule @{thm sngr_assn_def} *}
 lemma sngr_assn_rule [rewrite]:
   "(h, as) \<Turnstile> r \<mapsto>\<^sub>r x \<longleftrightarrow> (Ref.get h r = x \<and> as = {addr_of_ref r} \<and> addr_of_ref r < lim h)" by auto2
 setup {* del_prfstep_thm @{thm sngr_assn_def} *}
 
-definition snga_assn :: "'a::heap array \<Rightarrow> 'a list \<Rightarrow> assn" (infix "\<mapsto>\<^sub>a" 82) where
+definition snga_assn :: "'a::heap array \<Rightarrow> 'a list \<Rightarrow> assn" (infix "\<mapsto>\<^sub>a" 82) where [rewrite]:
   "r \<mapsto>\<^sub>a x = Abs_assn (Assn (
-    \<lambda>h. Array.get (fst h) r = x \<and> snd h = {addr_of_array r} \<and> addr_of_array r < lim (fst h)))"
+    \<lambda>(h, as). Array.get h r = x \<and> as = {addr_of_array r} \<and> addr_of_array r < lim h))"
 
-setup {* add_rewrite_rule @{thm snga_assn_def} *}
 lemma snga_assn_rule [rewrite]:
   "(h, as) \<Turnstile> r \<mapsto>\<^sub>a x \<longleftrightarrow> (Array.get h r = x \<and> as = {addr_of_array r} \<and> addr_of_array r < lim h)" by auto2
 setup {* del_prfstep_thm @{thm snga_assn_def} *}
 
-subsubsection {* Pure Assertions *}
+subsection {* Pure Assertions *}
 
-text {* Pure assertions do not depend on any heap content. *}
-
-definition pure_assn :: "bool \<Rightarrow> assn" ("\<up>") where
+definition pure_assn :: "bool \<Rightarrow> assn" ("\<up>") where [rewrite]:
   "\<up>b = Abs_assn (Assn (\<lambda>h. snd h = {} \<and> b))"
 
-setup {* add_rewrite_rule @{thm pure_assn_def} *}
 lemma pure_assn_rule [rewrite]: "h \<Turnstile> \<up>b \<longleftrightarrow> (snd h = {} \<and> b)" by auto2
 setup {* del_prfstep_thm @{thm pure_assn_def} *}
 
-definition top_assn :: assn ("true") where
+definition top_assn :: assn ("true") where [rewrite]:
   "top_assn = Abs_assn (Assn in_range)"
 
-setup {* add_rewrite_rule @{thm top_assn_def} *}
-theorem top_assn_rule [rewrite]: "h \<Turnstile> true \<longleftrightarrow> in_range h" by auto2
+lemma top_assn_rule [rewrite]: "h \<Turnstile> true \<longleftrightarrow> in_range h" by auto2
 setup {* del_prfstep_thm @{thm top_assn_def} *}
+
 setup {* del_prfstep_thm @{thm models_def} *}
+
+subsection {* Properties of assertions *}
 
 abbreviation bot_assn :: assn ("false") where "bot_assn \<equiv> \<up>False"
 
-lemma star_false_left [rewrite]: "false * P = false" by auto2
+lemma mod_false' [resolve]: "\<not> (h \<Turnstile> false * Ru)" by auto2
 
 lemma mod_star_trueI: "h \<Turnstile> P \<Longrightarrow> h \<Turnstile> P * true"
 @proof @have "set_partition (snd h) (snd h) {}" @qed
 
-theorem sngr_same_false [resolve]: "\<not>h \<Turnstile> p \<mapsto>\<^sub>r x * p \<mapsto>\<^sub>r y * Qu" by auto2
-theorem snga_same_false [resolve]: "\<not>h \<Turnstile> p \<mapsto>\<^sub>r x * p \<mapsto>\<^sub>r y * Qu" by auto2
+lemma sngr_same_false [resolve]: "\<not>h \<Turnstile> p \<mapsto>\<^sub>r x * p \<mapsto>\<^sub>r y * Qu" by auto2
 
-lemma mod_pure_star_dist [rewrite]: "h \<Turnstile> P * \<up>b \<longleftrightarrow> (h \<Turnstile> P \<and> b)"
-@proof @case "h \<Turnstile> P \<and> b" @with @have "set_partition (snd h) (snd h) {}" @end @qed
-
-lemma mod_pure' [rewrite]: "h \<Turnstile> \<up>b \<longleftrightarrow> (h \<Turnstile> emp \<and> b)" by auto2
-
-theorem ref_prec:
-  "h \<Turnstile> p \<mapsto>\<^sub>r x * Qu \<Longrightarrow> h \<Turnstile> p \<mapsto>\<^sub>r y * Ru \<Longrightarrow> x = y" by auto2
+lemma ref_prec: "h \<Turnstile> p \<mapsto>\<^sub>r x * Qu \<Longrightarrow> h \<Turnstile> p \<mapsto>\<^sub>r y * Ru \<Longrightarrow> x = y" by auto2
 setup {* add_forward_prfstep_cond @{thm ref_prec} [with_cond "?x \<noteq> ?y"] *}
 
-theorem array_ref_prec:
-  "h \<Turnstile> p \<mapsto>\<^sub>a x * Qu \<Longrightarrow> h \<Turnstile> p \<mapsto>\<^sub>a y * Ru \<Longrightarrow> x = y" by auto2
-setup {* add_forward_prfstep_cond @{thm array_ref_prec} [with_cond "?x \<noteq> ?y"] *}
+lemma array_prec: "h \<Turnstile> p \<mapsto>\<^sub>a x * Qu \<Longrightarrow> h \<Turnstile> p \<mapsto>\<^sub>a y * Ru \<Longrightarrow> x = y" by auto2
+setup {* add_forward_prfstep_cond @{thm array_prec} [with_cond "?x \<noteq> ?y"] *}
 
-theorem entailsD' [forward]: "P \<Longrightarrow>\<^sub>A Q \<Longrightarrow> h \<Turnstile> P * R \<Longrightarrow> h \<Turnstile> Q * R" by auto2
+lemma mod_pure_star_dist [rewrite]:
+  "h \<Turnstile> P * \<up>b \<longleftrightarrow> (h \<Turnstile> P \<and> b)"
+@proof
+  @case "h \<Turnstile> P \<and> b" @with
+    @have "set_partition (snd h) (snd h) {}"
+  @end
+@qed
+
+lemma mod_pure': "h \<Turnstile> \<up>b \<longleftrightarrow> (h \<Turnstile> emp \<and> b)" by auto2
+lemma pure_conj:  "\<up>(P \<and> Q) = \<up>P * \<up>Q" by auto2
+
+subsection {* Entailment and its properties *}
+
+definition entails :: "assn \<Rightarrow> assn \<Rightarrow> bool" (infix "\<Longrightarrow>\<^sub>A" 10) where [rewrite]:
+  "(P \<Longrightarrow>\<^sub>A Q) \<longleftrightarrow> (\<forall>h. h \<Turnstile> P \<longrightarrow> h \<Turnstile> Q)"
+
+lemma entails_triv: "A \<Longrightarrow>\<^sub>A A" by auto2
+lemma entails_true: "A \<Longrightarrow>\<^sub>A true" by auto2
+lemma entail_equiv_forward: "P = Q \<Longrightarrow> P \<Longrightarrow>\<^sub>A Q" by auto2
+lemma entail_equiv_backward: "P = Q \<Longrightarrow> Q \<Longrightarrow>\<^sub>A P" by auto2
+lemma entailsD [forward]: "P \<Longrightarrow>\<^sub>A Q \<Longrightarrow> h \<Turnstile> P \<Longrightarrow> h \<Turnstile> Q" by auto2
+lemma entailsD': "P \<Longrightarrow>\<^sub>A Q \<Longrightarrow> h \<Turnstile> P * R \<Longrightarrow> h \<Turnstile> Q * R" by auto2
+lemma entailsD_back: "P \<Longrightarrow>\<^sub>A Q \<Longrightarrow> \<not>h \<Turnstile> Q * R \<Longrightarrow> \<not>h \<Turnstile> P * R" by auto2
+lemma entail_trans2: "A \<Longrightarrow>\<^sub>A D * B \<Longrightarrow> B \<Longrightarrow>\<^sub>A C \<Longrightarrow> A \<Longrightarrow>\<^sub>A D * C" by auto2
+lemma entail_trans2': "D * B \<Longrightarrow>\<^sub>A A \<Longrightarrow> C \<Longrightarrow>\<^sub>A B \<Longrightarrow> D * C \<Longrightarrow>\<^sub>A A" by auto2
+lemma entails_invD: "A \<Longrightarrow>\<^sub>A B \<Longrightarrow> \<not>(h \<Turnstile> B) \<Longrightarrow> \<not>(h \<Turnstile> A)" by auto2
 
 section {* Definition of the run predicate *}
 
 inductive run :: "'a Heap \<Rightarrow> heap option \<Rightarrow> heap option \<Rightarrow> 'a \<Rightarrow> bool" where
-  "run c None None r " |
-  "execute c h = None \<Longrightarrow> run c (Some h) None r" |
-  "execute c h = Some (r, h') \<Longrightarrow> run c (Some h) (Some h') r"
+  "run c None None r"
+| "execute c h = None \<Longrightarrow> run c (Some h) None r"
+| "execute c h = Some (r, h') \<Longrightarrow> run c (Some h) (Some h') r"
 setup {* add_case_induct_rule @{thm run.cases} *}
 setup {* fold add_resolve_prfstep @{thms run.intros(1,2)} *}
 setup {* add_forward_prfstep @{thm run.intros(3)} *}
+setup {* add_backward_prfstep @{thm run.intros(3)} *}
 
-theorem run_preserve_None [forward]:
+lemma run_preserve_None [forward]:
   "run c None \<sigma>' r \<Longrightarrow> \<sigma>' = None"
 @proof @case_induct "run c None \<sigma>' r" @qed
 
-theorem run_execute_fail [forward]:
+lemma run_execute_fail [forward]:
   "execute c h = None \<Longrightarrow> run c (Some h) \<sigma>' r \<Longrightarrow> \<sigma>' = None"
 @proof @case_induct "run c (Some h) \<sigma>' r" @qed
 
-theorem run_execute_succeed [forward]:
+lemma run_execute_succeed [forward]:
   "execute c h = Some (r', h') \<Longrightarrow> run c (Some h) \<sigma>' r \<Longrightarrow> \<sigma>' = Some h' \<and> r = r'"
 @proof @case_induct "run c (Some h) \<sigma>' r" @qed
 
@@ -267,11 +257,9 @@ lemma run_complete [resolve]:
   @case "execute c (the \<sigma>) = None" @with @have "run c \<sigma> None r" @end
 @qed
 
-theorem run_to_execute [forward]:
+lemma run_to_execute [forward]:
   "run c (Some h) \<sigma>' r \<Longrightarrow> if \<sigma>' = None then execute c h = None else execute c h = Some (r, the \<sigma>')"
 @proof @case_induct "run c (Some h) \<sigma>' r" @qed
-
-setup {* add_backward_prfstep @{thm run.intros(3)} *}
 
 setup {* add_rewrite_rule @{thm execute_bind(1)} *}
 lemma runE [forward]:
@@ -282,39 +270,18 @@ setup {* add_rewrite_rule @{thm Array.get_alloc} *}
 setup {* add_rewrite_rule @{thm Ref.get_alloc} *}
 setup {* add_rewrite_rule_bidir @{thm Array.length_def} *}
 
-setup {* add_rewrite_rule @{thm execute_assert(1)} *}
-lemma execute_return': "execute (return x) h = Some (x, h)" by (metis comp_eq_dest_lhs execute_return)
-setup {* add_rewrite_rule @{thm execute_return'} *}
-setup {* add_rewrite_rule @{thm execute_len} *}
-setup {* add_rewrite_rule @{thm execute_new} *}
-setup {* add_rewrite_rule @{thm execute_of_list} *}
-setup {* add_rewrite_rule @{thm execute_upd(1)} *}
-setup {* add_rewrite_rule @{thm execute_ref} *}
-setup {* add_rewrite_rule @{thm execute_lookup} *}
-setup {* add_rewrite_rule @{thm execute_nth(1)} *}
-setup {* add_rewrite_rule @{thm execute_update} *}
-
 section {* Definition of hoare triple, and the frame rule. *}
 
-text {* Analyze the heap before and after executing a command, to add
-  the allocated addresses to the covered address range. *}
-
-definition new_addrs :: "heap \<Rightarrow> addr set \<Rightarrow> heap \<Rightarrow> addr set" where
+definition new_addrs :: "heap \<Rightarrow> addr set \<Rightarrow> heap \<Rightarrow> addr set" where [rewrite]:
   "new_addrs h as h' = as \<union> {a. lim h \<le> a \<and> a < lim h'}"
-setup {* add_rewrite_rule @{thm new_addrs_def} *}
 
 lemma new_addr_refl [rewrite]: "new_addrs h as h = as" by auto2
 
-definition hoare_triple :: "assn \<Rightarrow> 'a Heap \<Rightarrow> ('a \<Rightarrow> assn) \<Rightarrow> bool" ("<_>/ _/ <_>") where
+definition hoare_triple :: "assn \<Rightarrow> 'a Heap \<Rightarrow> ('a \<Rightarrow> assn) \<Rightarrow> bool" ("<_>/ _/ <_>") where [rewrite]:
   "<P> c <Q> \<longleftrightarrow> (\<forall>h as \<sigma> r. (h, as) \<Turnstile> P \<longrightarrow> run c (Some h) \<sigma> r \<longrightarrow>
     (\<sigma> \<noteq> None \<and> (the \<sigma>, new_addrs h as (the \<sigma>)) \<Turnstile> Q r \<and> relH {a . a < lim h \<and> a \<notin> as} h (the \<sigma>) \<and>
      lim h \<le> lim (the \<sigma>)))"
-setup {* add_forward_prfstep (equiv_forward_th @{thm hoare_triple_def}) *}
-setup {* add_resolve_prfstep (equiv_backward_th @{thm hoare_triple_def}) *}
 
-text {* For garbage-collected languages, specifications usually allow for some
-  arbitrary heap parts in the postcondition. The following abbreviation defines
-  a handy shortcut notation for such specifications. *}
 abbreviation hoare_triple' :: "assn \<Rightarrow> 'r Heap \<Rightarrow> ('r \<Rightarrow> assn) \<Rightarrow> bool" ("<_> _ <_>\<^sub>t") where
   "<P> c <Q>\<^sub>t \<equiv> <P> c <\<lambda>r. Q r * true>"
 
@@ -332,88 +299,91 @@ lemma frame_rule [backward]:
 
 (* This is the last use of the definition of separating conjunction. *)
 setup {* del_prfstep_thm @{thm mod_star_conv} *}
-setup {* del_prfstep_thm_str "@eqbackward@res" @{thm hoare_triple_def} *}
+
+lemma norm_pre_pure_iff: "<P * \<up>b> c <Q> \<longleftrightarrow> (b \<longrightarrow> <P> c <Q>)" by auto2
 
 section {* Hoare triples for atomic commands *}
 
-setup {* add_backward_prfstep (equiv_backward_th @{thm hoare_triple_def}) *}
-
 (* First, those that do not modify the heap. *)
-
-(* Avoid variables P and Q since they are pre- and post-condition. *)
-
+setup {* add_rewrite_rule @{thm execute_assert(1)} *}
 lemma assert_rule:
   "<\<up>(R x)> assert R x <\<lambda>r. \<up>(r = x)>" by auto2
 
+lemma execute_return' [rewrite]: "execute (return x) h = Some (x, h)" by (metis comp_eq_dest_lhs execute_return)
 lemma return_rule:
   "<emp> return x <\<lambda>r. \<up>(r = x)>" by auto2
 
+setup {* add_rewrite_rule @{thm execute_nth(1)} *}
 lemma nth_rule:
   "<a \<mapsto>\<^sub>a xs * \<up>(i < length xs)> Array.nth a i <\<lambda>r. a \<mapsto>\<^sub>a xs * \<up>(r = xs ! i)>" by auto2
 
+setup {* add_rewrite_rule @{thm execute_len} *}
 lemma length_rule:
   "<a \<mapsto>\<^sub>a xs> Array.len a <\<lambda>r. a \<mapsto>\<^sub>a xs * \<up>(r = length xs)>" by auto2
 
+setup {* add_rewrite_rule @{thm execute_lookup} *}
 lemma lookup_rule:
   "<p \<mapsto>\<^sub>r x> !p <\<lambda>r. p \<mapsto>\<^sub>r x * \<up>(r = x)>" by auto2
 
 (* Next, the update rules. *)
 setup {* add_rewrite_rule @{thm Ref.lim_set} *}
-theorem Array_lim_set [rewrite]: "lim (Array.set p xs h) = lim h" by (simp add: Array.set_def)
+lemma Array_lim_set [rewrite]: "lim (Array.set p xs h) = lim h" by (simp add: Array.set_def)
 
 setup {* fold add_rewrite_rule [@{thm Ref.get_set_eq}, @{thm Array.get_set_eq}] *}
 setup {* add_rewrite_rule @{thm Array.update_def} *}
 
+setup {* add_rewrite_rule @{thm execute_upd(1)} *}
 lemma upd_rule:
   "<a \<mapsto>\<^sub>a xs * \<up>(i < length xs)> Array.upd i x a <\<lambda>r. a \<mapsto>\<^sub>a list_update xs i x * \<up>(r = a)>" by auto2
 
+setup {* add_rewrite_rule @{thm execute_update} *}
 lemma update_rule:
   "<p \<mapsto>\<^sub>r y> p := x <\<lambda>r. p \<mapsto>\<^sub>r x>" by auto2
 
 (* Finally, the allocation rules. *)
-theorem lim_set_gen [rewrite]: "lim (h\<lparr>lim := l\<rparr>) = l" by simp
+lemma lim_set_gen [rewrite]: "lim (h\<lparr>lim := l\<rparr>) = l" by simp
 
-theorem Array_alloc_def' [rewrite]: 
+lemma Array_alloc_def' [rewrite]: 
   "Array.alloc xs h = (let l = lim h; r = Array l in (r, (Array.set r xs (h\<lparr>lim := l + 1\<rparr>))))"
   by (simp add: Array.alloc_def)
 
 setup {* fold add_rewrite_rule [
   @{thm addr_of_array.simps}, @{thm addr_of_ref.simps}, @{thm Ref.alloc_def}] *}
 
-theorem refs_on_Array_set [rewrite]: "refs (Array.set p xs h) t i = refs h t i"
+lemma refs_on_Array_set [rewrite]: "refs (Array.set p xs h) t i = refs h t i"
   by (simp add: Array.set_def)
 
-theorem arrays_on_Ref_set [rewrite]: "arrays (Ref.set p x h) t i = arrays h t i"
+lemma arrays_on_Ref_set [rewrite]: "arrays (Ref.set p x h) t i = arrays h t i"
   by (simp add: Ref.set_def)
 
-theorem refs_on_Array_alloc [rewrite]: "refs (snd (Array.alloc xs h)) t i = refs h t i"
+lemma refs_on_Array_alloc [rewrite]: "refs (snd (Array.alloc xs h)) t i = refs h t i"
   by (metis (no_types, lifting) Array.alloc_def refs_on_Array_set select_convs(2) snd_conv surjective update_convs(3))
 
-theorem arrays_on_Ref_alloc [rewrite]: "arrays (snd (Ref.alloc x h)) t i = arrays h t i"
+lemma arrays_on_Ref_alloc [rewrite]: "arrays (snd (Ref.alloc x h)) t i = arrays h t i"
   by (metis (no_types, lifting) Ref.alloc_def arrays_on_Ref_set select_convs(1) sndI surjective update_convs(3))
 
-theorem arrays_on_Array_alloc [rewrite]: "i < lim h \<Longrightarrow> arrays (snd (Array.alloc xs h)) t i = arrays h t i"
+lemma arrays_on_Array_alloc [rewrite]: "i < lim h \<Longrightarrow> arrays (snd (Array.alloc xs h)) t i = arrays h t i"
   by (smt Array.alloc_def Array.set_def addr_of_array.simps fun_upd_apply less_or_eq_imp_le
           linorder_not_less simps(1) snd_conv surjective update_convs(1) update_convs(3))
 
-theorem refs_on_Ref_alloc [rewrite]: "i < lim h \<Longrightarrow> refs (snd (Ref.alloc x h)) t i = refs h t i"
+lemma refs_on_Ref_alloc [rewrite]: "i < lim h \<Longrightarrow> refs (snd (Ref.alloc x h)) t i = refs h t i"
   by (smt Ref.alloc_def Ref.set_def addr_of_ref.simps fun_upd_apply less_or_eq_imp_le
           linorder_not_less select_convs(2) simps(6) snd_conv surjective update_convs(3))
 
+setup {* add_rewrite_rule @{thm execute_new} *}
 lemma new_rule:
   "<emp> Array.new n x <\<lambda>r. r \<mapsto>\<^sub>a replicate n x>" by auto2
 
+setup {* add_rewrite_rule @{thm execute_of_list} *}
 lemma of_list_rule:
   "<emp> Array.of_list xs <\<lambda>r. r \<mapsto>\<^sub>a xs>" by auto2
 
+setup {* add_rewrite_rule @{thm execute_ref} *}
 lemma ref_rule:
   "<emp> ref x <\<lambda>r. r \<mapsto>\<^sub>r x>" by auto2
 
 setup {* fold del_prfstep_thm [@{thm sngr_assn_rule}, @{thm snga_assn_rule}] *}
-
-section {* Other properties *}
-
-theorem norm_pre_pure_iff: "<P * \<up>b> c <Q> \<longleftrightarrow> (b \<longrightarrow> <P> c <Q>)" by auto2
+setup {* fold del_prfstep_thm [@{thm pure_assn_rule}, @{thm top_assn_rule}, @{thm mod_pure_star_dist}] *}
 
 section {* success_run and its properties. *}
 
@@ -425,89 +395,68 @@ fun success_run :: "'a Heap \<Rightarrow> pheap \<Rightarrow> pheap \<Rightarrow
     as' = new_addrs h as h' \<and> run f (Some h) (Some h') r \<and> relH {a. a < lim h \<and> a \<notin> as} h h' \<and> lim h \<le> lim h'"
 setup {* add_rewrite_rule @{thm success_run.simps} *}
 
-theorem success_run_bind:
+lemma success_run_bind:
   "success_run f h h' r \<Longrightarrow> success_run (g r) h' h'' r' \<Longrightarrow> success_run (f \<bind> g) h h'' r'" by auto2
 
-theorem success_run_next: "success_run f h h'' r' \<Longrightarrow>
+lemma success_run_next: "success_run f h h'' r' \<Longrightarrow>
   \<forall>h'. \<sigma> = Some (fst h') \<and> success_run (f \<bind> g) h h' r \<longrightarrow> \<not> h' \<Turnstile> Q \<Longrightarrow>
   \<forall>h'. \<sigma> = Some (fst h') \<and> success_run (g r') h'' h' r \<longrightarrow> \<not> h' \<Turnstile> Q" by auto2
 
-theorem hoare_triple_def' [rewrite]:
+lemma hoare_triple_def' [rewrite]:
   "<P> c <Q> \<longleftrightarrow> (\<forall>h \<sigma> r. h \<Turnstile> P \<longrightarrow> run c (Some (fst h)) \<sigma> r \<longrightarrow>
-    (\<sigma> \<noteq> None \<and> (the \<sigma>, new_addrs (fst h) (snd h) (the \<sigma>)) \<Turnstile> Q r \<and> relH {a . a < lim (fst h) \<and> a \<notin> (snd h)} (fst h) (the \<sigma>) \<and>
+    (\<sigma> \<noteq> None \<and> (the \<sigma>, new_addrs (fst h) (snd h) (the \<sigma>)) \<Turnstile> Q r \<and>
+     relH {a . a < lim (fst h) \<and> a \<notin> (snd h)} (fst h) (the \<sigma>) \<and>
      lim (fst h) \<le> lim (the \<sigma>)))" using hoare_triple_def by fastforce
 
-theorem hoare_tripleE': "<P> c <Q> \<Longrightarrow> h \<Turnstile> P * Ru \<Longrightarrow> run c (Some (fst h)) \<sigma> r \<Longrightarrow>
-  \<exists>h'. h' \<Turnstile> Q r * Ru \<and> \<sigma> = Some (fst h') \<and> success_run c h h' r"
+lemma hoare_tripleE':
+  "<P> c <Q> \<Longrightarrow> h \<Turnstile> P * Ru \<Longrightarrow> run c (Some (fst h)) \<sigma> r \<Longrightarrow>
+   \<exists>h'. h' \<Turnstile> Q r * Ru \<and> \<sigma> = Some (fst h') \<and> success_run c h h' r"
 @proof @have "<P * Ru> c <\<lambda>r. Q r * Ru>" @qed
 
-theorem hoare_tripleI: "\<not><P> c <Q> \<Longrightarrow> \<exists>h \<sigma> r. h \<Turnstile> P \<and> run c (Some (fst h)) \<sigma> r \<and>
-  (\<forall>h'. \<sigma> = Some (fst h') \<and> success_run c h h' r \<longrightarrow> \<not>h' \<Turnstile> Q r)" by auto2
+lemma hoare_tripleI:
+  "\<not><P> c <Q> \<Longrightarrow> \<exists>h \<sigma> r. h \<Turnstile> P \<and> run c (Some (fst h)) \<sigma> r \<and>
+   (\<forall>h'. \<sigma> = Some (fst h') \<and> success_run c h h' r \<longrightarrow> \<not>h' \<Turnstile> Q r)" by auto2
 
-theorem hoare_triple_mp: "<P> c <Q> \<Longrightarrow> h \<Turnstile> P * Ru \<Longrightarrow> success_run c h h' r \<Longrightarrow> h' \<Turnstile> (Q r) * Ru"
+lemma hoare_triple_mp:
+  "<P> c <Q> \<Longrightarrow> h \<Turnstile> P * Ru \<Longrightarrow> success_run c h h' r \<Longrightarrow> h' \<Turnstile> (Q r) * Ru"
 @proof @have "<P * Ru> c <\<lambda>r. Q r * Ru>" @qed
 
-theorem hoare_tripleE'': "<P> c <Q> \<Longrightarrow> h \<Turnstile> P * Ru \<Longrightarrow> run (c \<bind> g) (Some (fst h)) \<sigma> r \<Longrightarrow>
-  \<exists>r' h'. run (g r') (Some (fst h')) \<sigma> r \<and> h' \<Turnstile> Q r' * Ru \<and> success_run c h h' r'"
+lemma hoare_tripleE'':
+  "<P> c <Q> \<Longrightarrow> h \<Turnstile> P * Ru \<Longrightarrow> run (c \<bind> g) (Some (fst h)) \<sigma> r \<Longrightarrow>
+   \<exists>r' h'. run (g r') (Some (fst h')) \<sigma> r \<and> h' \<Turnstile> Q r' * Ru \<and> success_run c h h' r'"
 @proof
   @have "<P * Ru> c <\<lambda>r. Q r * Ru>" @then
   @obtain \<sigma>' r' where "run c (Some (fst h)) \<sigma>' r'"
 @qed
 
-definition heap_preserving :: "'a Heap \<Rightarrow> bool" where
+definition heap_preserving :: "'a Heap \<Rightarrow> bool" where [rewrite]:
   "heap_preserving c = (\<forall>h h' r. effect c h h' r \<longrightarrow> h = h')"
-setup {* add_rewrite_rule @{thm heap_preserving_def} *}
 
 setup {* add_forward_prfstep @{thm effectI} *}
-
-theorem heap_preservingD [forward]:
+lemma heap_preservingD [forward]:
   "heap_preserving c \<Longrightarrow> success_run c h h' r \<Longrightarrow> h = h'" by auto2
+setup {* del_prfstep_thm @{thm effectI} *}
 
-theorem heap_preserving_effectD:
+lemma heap_preserving_effectD:
   "heap_preserving c \<Longrightarrow> effect c h h' r \<Longrightarrow> h = h'" by auto2
 
-theorem effect_bind [forward]: "effect (f \<bind> g) h h'' r' \<Longrightarrow> \<exists>h' r. effect f h h' r \<and> effect (g r) h' h'' r'"
+lemma effect_bind [forward]:
+  "effect (f \<bind> g) h h'' r' \<Longrightarrow> \<exists>h' r. effect f h h' r \<and> effect (g r) h' h'' r'"
   by (elim effect_elims) auto
 
-theorem hoare_tripleE'_preserve: "heap_preserving c \<Longrightarrow>
-  \<exists>h'. h' \<Turnstile> Q \<and> \<sigma> = Some (fst h') \<and> success_run c h h' r \<Longrightarrow>
-  h \<Turnstile> Q \<and> \<sigma> = Some (fst h) \<and> success_run c h h r" by auto2
+lemma hoare_tripleE'_preserve:
+  "heap_preserving c \<Longrightarrow>
+   \<exists>h'. h' \<Turnstile> Q \<and> \<sigma> = Some (fst h') \<and> success_run c h h' r \<Longrightarrow>
+   h \<Turnstile> Q \<and> \<sigma> = Some (fst h) \<and> success_run c h h r" by auto2
 
-theorem hoare_tripleE''_preserve: "heap_preserving c \<Longrightarrow>
-  \<exists>r' h'. run (g r') (Some (fst h')) \<sigma> r \<and> h' \<Turnstile> Q r' * Ru \<and> success_run c h h' r' \<Longrightarrow>
-  \<exists>r'. run (g r') (Some (fst h)) \<sigma> r \<and> h \<Turnstile> Q r' * Ru \<and> success_run c h h r'" by auto2
+lemma hoare_tripleE''_preserve:
+  "heap_preserving c \<Longrightarrow>
+   \<exists>r' h'. run (g r') (Some (fst h')) \<sigma> r \<and> h' \<Turnstile> Q r' * Ru \<and> success_run c h h' r' \<Longrightarrow>
+   \<exists>r'. run (g r') (Some (fst h)) \<sigma> r \<and> h \<Turnstile> Q r' * Ru \<and> success_run c h h r'" by auto2
 
-setup {* del_prfstep_thm @{thm effectI} *}
+setup {* del_prfstep_thm @{thm success_run.simps} *}
 setup {* del_prfstep_thm @{thm hoare_triple_def} *}
 setup {* del_prfstep_thm @{thm hoare_triple_def'} *}
-setup {* del_prfstep_thm @{thm success_run.simps} *}
-
-subsection {* Assertions *}
-
-lemma pure_conj:  "\<up>(P \<and> Q) = \<up>P * \<up>Q" by auto2
-lemma mod_false' [resolve]: "\<not> (h \<Turnstile> false * Ru)" by auto2
-
-subsection {* Entailment *}
-
-lemma entails_true: "A \<Longrightarrow>\<^sub>A true" by auto2
-lemma entail_equiv_forward: "P = Q \<Longrightarrow> P \<Longrightarrow>\<^sub>A Q" by auto2
-lemma entail_equiv_backward: "P = Q \<Longrightarrow> Q \<Longrightarrow>\<^sub>A P" by auto2
-lemma entailsD_back: "P \<Longrightarrow>\<^sub>A Q \<Longrightarrow> \<not>h \<Turnstile> Q * R \<Longrightarrow> \<not>h \<Turnstile> P * R" by auto2
-lemma entails_triv: "A \<Longrightarrow>\<^sub>A A" by auto2
-lemma entail_trans2: "A \<Longrightarrow>\<^sub>A D * B \<Longrightarrow> B \<Longrightarrow>\<^sub>A C \<Longrightarrow> A \<Longrightarrow>\<^sub>A D * C"
-  by (simp add: assn_times_comm entailsD' entails_def)
-lemma entail_trans2': "D * B \<Longrightarrow>\<^sub>A A \<Longrightarrow> C \<Longrightarrow>\<^sub>A B \<Longrightarrow> D * C \<Longrightarrow>\<^sub>A A"
-  by (simp add: assn_times_comm entailsD' entails_def)
-lemma entails_invD: "A \<Longrightarrow>\<^sub>A B \<Longrightarrow> \<not>(h \<Turnstile> B) \<Longrightarrow> \<not>(h \<Turnstile> A)"
-  using entailsD by blast
-
-lemma mod_array_eq [backward1]: "xs = xs' \<Longrightarrow> h \<Turnstile> p \<mapsto>\<^sub>a xs \<Longrightarrow> h \<Turnstile> p \<mapsto>\<^sub>a xs'" by simp
-
-subsection {* Clear unused proofsteps *}
-
-setup {* fold del_prfstep_thm [
-  @{thm mod_ex_dist}, @{thm ex_assn_def}, @{thm pure_assn_rule}, @{thm top_assn_rule},
-  @{thm star_false_left}, @{thm entailsD'}, @{thm mod_pure_star_dist}, @{thm mod_pure'}] *}
 
 subsection {* Definition of procedures *}
 
@@ -517,7 +466,7 @@ named_theorems sep_prec_thms "Seplogic: precision theorems"
 named_theorems sep_heap_presv_thms "Seplogic: heap preservation theorems"
 
 declare ref_prec [sep_prec_thms]
-declare array_ref_prec [sep_prec_thms]
+declare array_prec [sep_prec_thms]
 
 (* ASCII abbreviations for ML files. *)
 abbreviation (input) ex_assn_ascii :: "('a \<Rightarrow> assn) \<Rightarrow> assn" (binder "EXA" 11)
